src/GoExtraction.v
@@ -60,12 +60,11 @@ Ltac do_declare T cont :=
   lazymatch goal with
   | [ |- EXTRACT _ {{ ?pre }} _ {{ _ }} // _ ] =>
     lazymatch pre with
-    | context [decls_pre ?decls ?vars] =>
+    | context [decls_pre ?decls ?vars ?m] =>
       let decls' := fresh "decls" in
       evar (decls' : list Declaration);
       unify decls (Decl T :: decls'); subst decls';
-      cont (@snd (n_tuple_unit
-        (@Datatypes.length _ _) _) _ vars)
+      cont (pair_vec_nthl 0 m vars)
     end
   end.
 
